src/compiler/meta/OCL_compiler_parser_UML.thy
@@ -80,7 +80,8 @@ definition "ocl_class_raw_rec0 f ocl = f
   (ClassRaw_name ocl)
   (ClassRaw_own ocl)
   (ClassRaw_contract ocl)
-  (ClassRaw_invariant ocl)"
+  (ClassRaw_invariant ocl)
+  (ClassRaw_abstract ocl)"
 
 definition "ocl_class_raw_rec f ocl = ocl_class_raw_rec0 f ocl
   (ocl_class_raw.more ocl)"
@@ -112,19 +113,19 @@ definition "ocl_ctxt_inv_rec f ocl = ocl_ctxt_inv_rec0 f ocl
 
 (* *)
 
-lemma [code]: "ocl_class_raw.extend = (\<lambda>ocl v. ocl_class_raw_rec0 (co4 (\<lambda>f. f v) ocl_class_raw_ext) ocl)"
+lemma [code]: "ocl_class_raw.extend = (\<lambda>ocl v. ocl_class_raw_rec0 (co5 (\<lambda>f. f v) ocl_class_raw_ext) ocl)"
 by(intro ext, simp add: ocl_class_raw_rec0_def
                         ocl_class_raw.extend_def
-                        co4_def K_def)
-lemma [code]: "ocl_class_raw.make = co4 (\<lambda>f. f ()) ocl_class_raw_ext"
+                        co5_def K_def)
+lemma [code]: "ocl_class_raw.make = co5 (\<lambda>f. f ()) ocl_class_raw_ext"
 by(intro ext, simp add: ocl_class_raw.make_def
-                        co4_def)
-lemma [code]: "ocl_class_raw.truncate = ocl_class_raw_rec (co4 K ocl_class_raw.make)"
+                        co5_def)
+lemma [code]: "ocl_class_raw.truncate = ocl_class_raw_rec (co5 K ocl_class_raw.make)"
 by(intro ext, simp add: ocl_class_raw_rec0_def
                         ocl_class_raw_rec_def
                         ocl_class_raw.truncate_def
                         ocl_class_raw.make_def
-                        co4_def K_def)
+                        co5_def K_def)
 
 lemma [code]: "ocl_association.extend = (\<lambda>ocl v. ocl_association_rec0 (co2 (\<lambda>f. f v) ocl_association_ext) ocl)"
 by(intro ext, simp add: ocl_association_rec0_def
@@ -186,7 +187,10 @@ definition "i_of_ocl_ty_obj_core a b = rec_ocl_ty_obj_core
 definition "i_of_ocl_ty_obj a b = rec_ocl_ty_obj
   (ap2 a (b \<open>OclTyObj\<close>) (i_of_ocl_ty_obj_core a b) (i_of_list a b (i_of_list a b (i_of_ocl_ty_obj_core a b))))"
 
-definition "i_of_ocl_ty a b = (\<lambda>f1 f2 f3 f4 f5 f6 f7 f8 f9. rec_ocl_ty f1 f2 f3 f4 f5 f6 f7 (K o f8) (\<lambda>_ _. f9))
+definition "i_of_ocl_ty a b = (\<lambda>f1 f2 f3 f4 f5 f6 f7 f8 f9 f10 f11 f12 f13 f14 f15.
+                                    rec_ocl_ty_1 f1 f2 f3 f4 f5 f6
+                                                 f7 (K o f8) (\<lambda>_ _. f9) (\<lambda>_. f10) (\<lambda>_ _. f11) f12
+                                                 (K o f13) (K o f14) (K o f15))
   (b \<open>OclTy_base_void\<close>)
   (b \<open>OclTy_base_boolean\<close>)
   (b \<open>OclTy_base_integer\<close>)
@@ -196,7 +200,13 @@ definition "i_of_ocl_ty a b = (\<lambda>f1 f2 f3 f4 f5 f6 f7 f8 f9. rec_ocl_ty f
   (ap1 a (b \<open>OclTy_object\<close>) (i_of_ocl_ty_obj a b))
   (ar2 a (b \<open>OclTy_collection\<close>) (i_of_ocl_multiplicity a b (K i_of_unit)))
   (ar2 a (b \<open>OclTy_pair\<close>) id)
-  (ap1 a (b \<open>OclTy_raw\<close>) (i_of_string a b))"
+  (ar1 a (b \<open>OclTy_pair1\<close>))
+  (ar2 a (b \<open>OclTy_arrow\<close>) id)
+  (ap1 a (b \<open>OclTy_raw\<close>) (i_of_string a b))
+  (* *)
+  (curry (i_of_pair a b (i_of_option a b (i_of_string a b)) id))
+  (curry (i_of_pair a b (i_of_option a b (i_of_string a b)) id))
+  (curry (i_of_pair a b (i_of_option a b (i_of_string a b)) id))"
 
 definition "i_of_ocl_association_type a b = rec_ocl_association_type
   (b \<open>OclAssTy_native_attribute\<close>)
@@ -207,7 +217,7 @@ definition "i_of_ocl_association_type a b = rec_ocl_association_type
 definition "i_of_ocl_association a b f = ocl_association_rec
   (ap3 a (b (ext \<open>ocl_association_ext\<close>))
     (i_of_ocl_association_type a b)
-    (i_of_list a b (i_of_pair a b (i_of_string a b) (i_of_ocl_multiplicity a b (K i_of_unit))))
+    (i_of_list a b (i_of_pair a b (i_of_ocl_ty_obj a b) (i_of_ocl_multiplicity a b (K i_of_unit))))
     (f a b))"
 
 definition "i_of_ocl_ctxt_prefix a b = rec_ocl_ctxt_prefix
@@ -244,11 +254,12 @@ definition "i_of_ocl_class a b = (\<lambda>f0 f1 f2 f3 f4. rec_ocl_class_1 (co2 
     (ar2 a (b i_Cons) id)"
 
 definition "i_of_ocl_class_raw a b f = ocl_class_raw_rec
-  (ap5 a (b (ext \<open>ocl_class_raw_ext\<close>))
+  (ap6 a (b (ext \<open>ocl_class_raw_ext\<close>))
     (i_of_ocl_ty_obj a b)
     (i_of_list a b (i_of_pair a b (i_of_string a b) (i_of_ocl_ty a b)))
     (i_of_list a b (i_of_ocl_ctxt_pre_post a b (K i_of_unit)))
     (i_of_list a b (i_of_ocl_ctxt_inv a b (K i_of_unit)))
+    (i_of_bool b)
     (f a b))"
 
 definition "i_of_ocl_ass_class a b = rec_ocl_ass_class
